src/Examples/StatDb.v
@@ -1,0 +1,57 @@
+Require Import RecoveryRefinement.POCS.
+From Coq Require Import List.
+
+Module Var.
+  Inductive id := Sum | Count.
+  Inductive Op : Type -> Type :=
+  | Read (i:id) : Op nat
+  | Write (i:id) (v:nat) : Op unit .
+  Definition State := (nat * nat)%type.
+
+  Definition get (i:id) : State -> nat :=
+    match i with
+    | Sum => fun '(x, _) => x
+    | Count => fun '(_, y) => y
+    end.
+
+  Definition set (i:id) (v:nat) : State -> State :=
+    match i with
+    | Sum => fun '(_, y) => (v, y)
+    | Count => fun '(x, _) => (x, v)
+    end.
+
+  Definition dynamics : Dynamics Op State :=
+    {| step T (op: Op T) :=
+         match op with
+         | Read i => reads (get i)
+         | Write i v => puts (set i v)
+         end;
+       crash_step :=
+         puts (fun _ => (0, 0)); |}.
+
+  Definition l : Layer Op :=
+    {| Layer.State := State;
+       sem := dynamics;
+       initP := fun s => s = (0, 0)|}.
+End Var.
+
+Module DB.
+  Inductive Op : Type -> Type :=
+  | Add (n:nat) : Op unit
+  | Avg : Op nat.
+  Definition State := list nat.
+
+  Definition dynamics : Dynamics Op State :=
+    {| step T (op: Op T) :=
+         match op with
+         | Add n => puts (cons n)
+         | Avg => reads (fun l => fold_left plus l 0 / length l)
+         end;
+       crash_step :=
+         puts (fun _ => nil); |}.
+
+  Definition l : Layer Op :=
+    {| Layer.State := State;
+       sem := dynamics;
+       initP := fun s => s = nil |}.
+End DB.
