src/POCS.v
@@ -2,6 +2,7 @@ From Coq Require Export List.
 From Coq Require Export Omega.
 
 Require Export Helpers.Instances.
+Require Export Helpers.RelationAlgebra.
 Require Export Tactical.ProofAutomation.
 
 Require Export Spec.Proc.
